cfrontend/PrintClight.ml
@@ -19,7 +19,7 @@
 open Format
 open Camlcoq
 open PrintAST
-open Ctypes
+open CTypes
 open Cop
 open PrintCsyntax
 open Clight
@@ -275,17 +275,17 @@ let print_function ver p id f =
 
 let print_fundef ver p id fd =
   match fd with
-  | Ctypes.External(_, _, _, _) ->
+  | CTypes.External(_, _, _, _) ->
       ()
   | Internal f ->
       print_function ver p id f
 
 let print_fundecl p id fd =
   match fd with
-  | Ctypes.External((AST.EF_external _ | AST.EF_runtime _ | AST.EF_malloc | AST.EF_free), args, res, cconv) ->
+  | CTypes.External((AST.EF_external _ | AST.EF_runtime _ | AST.EF_malloc | AST.EF_free), args, res, cconv) ->
       fprintf p "extern %s;@ "
                 (name_cdecl (extern_atom id) (Tfunction(args, res, cconv)))
-  | Ctypes.External(_, _, _, _) ->
+  | CTypes.External(_, _, _, _) ->
       ()
   | Internal f ->
       fprintf p "%s;@ "
