my/Prioritizer.ml
@@ -1,0 +1,32 @@
+open Ctypes
+
+let prioritize nodes n edges m =
+  (* First, we will need to convert them to C arrays *)
+  let nodes_arr = CArray.of_list int nodes in
+  let edges_arr =
+    let inner = List.map (fun e -> CArray.of_list int e |> CArray.start) edges in
+    let outer = CArray.of_list (ptr int) inner in
+    outer
+  in
+
+  let n = List.length nodes in
+  let m = List.length edges in
+
+
+  (* Now, we pass arguments into prioritizer *)
+  let result0 =
+    C.Functions.prioritizer (CArray.start nodes_arr) n (CArray.start edges_arr) m
+  in
+  let result1 =
+    C.Functions.prioritizer (CArray.start nodes_arr) n (CArray.start edges_arr) m
+  in
+
+  CArray.from_ptr result0 n
+  |> CArray.to_list
+  |> List.iteri (fun i x -> Format.printf "priority[%d] = %d\n" i x)
+  ;
+  CArray.from_ptr result1 n
+  |> CArray.to_list
+  |> List.iteri (fun i x -> Format.printf "priority[%d] = %d\n" i x)
+
+;;
