my/foo.c
@@ -1,0 +1,31 @@
+#include<stdlib.h>
+#include<stdio.h>
+
+int GLOBAL = 10;
+
+int int_id(int a) {
+  return a;
+}
+
+/*
+  Arguments
+   - nodes: 1-D array with size of n
+   - edges: 2-D array with size of m x 2
+  Return
+   - priority: 1-D array with size of n
+*/
+int *prioritizer(int *nodes, int n, int **edges, int m) {
+  int *priority = (int *) calloc(n, sizeof(int));
+
+  GLOBAL += 1;
+
+  /* Update priority array */
+
+  // TODO: replace with implementation of prioritizer
+  // For now, I simply output the reverse of nodes
+  for (int i = n-1; i >= 0 ; i--) {
+    priority[i] = GLOBAL + i;
+  }
+
+  return priority;
+}
