my/headers/foo.h
@@ -1,0 +1,3 @@
+int int_id(int);
+
+int *prioritizer(int*, int, int**, int);
