my/type_description.ml
@@ -1,0 +1,3 @@
+module Types (F : Ctypes.TYPE) = struct
+  (* Define any C library types and constants *)
+end
