cfrontend/Cexec.v
@@ -17,7 +17,7 @@ Require Import Axioms Classical.
 Require Import String Coqlib Decidableplus.
 Require Import Errors Maps Integers Floats.
 Require Import AST Values Memory Events Globalenvs Builtins Determinism.
-Require Import Ctypes Cop Csyntax Csem.
+Require Import CTypes Cop Csyntax Csem.
 Require Cstrategy.
 
 Local Open Scope string_scope.
