extraction/extraction.v
@@ -28,13 +28,14 @@ Require ValueDomain.
 Require Tailcall.
 Require Allocation.
 Require Bounds.
-Require Ctypes.
+Require CTypes.
 Require Csyntax.
 Require Ctyping.
 Require Clight.
 Require Compiler.
 Require Parser.
 Require Initializers.
+Require Scheduling.
 
 (* Standard lib *)
 Require Import ExtrOcamlBasic.
@@ -147,6 +148,8 @@ Extraction Blacklist List String Int.
 (* Needed in Coq 8.4 to avoid problems with Function definitions. *)
 Set Extraction AccessOpaque.
 
+Extract Constant Scheduling.prioritize => "Prioritizer.prioritize".
+
 (* Go! *)
 
 Cd "extraction".
@@ -154,14 +157,14 @@ Cd "extraction".
 Separate Extraction
    Compiler.transf_c_program Compiler.transf_cminor_program
    Cexec.do_initial_state Cexec.do_step Cexec.at_final_state
-   Ctypes.merge_attributes Ctypes.remove_attributes 
-   Ctypes.build_composite_env Ctypes.layout_struct
+   CTypes.merge_attributes CTypes.remove_attributes 
+   CTypes.build_composite_env CTypes.layout_struct
    Initializers.transl_init Initializers.constval
    Csyntax.Eindex Csyntax.Epreincr Csyntax.Eselection
    Ctyping.typecheck_program
    Ctyping.epostincr Ctyping.epostdecr Ctyping.epreincr Ctyping.epredecr
    Ctyping.eselection
-   Ctypes.make_program
+   CTypes.make_program
    Clight.type_of_function
    Conventions1.callee_save_type Conventions1.is_float_reg
    Conventions1.int_caller_save_regs Conventions1.float_caller_save_regs
